Montgomery.XZ, Loops: montladder proof scaffolding

src/Experiments/Loops.v
@@ -1,10 +1,14 @@
 Require Import Coq.Lists.List.
 Require Import Lia. 
-Require Import Crypto.Util.ListUtil.
+Require Import Crypto.Util.Tactics.UniquePose.
+Require Import Crypto.Util.Tactics.BreakMatch.
+Require Import Crypto.Util.Tactics.DestructHead.
 Require Import Crypto.Util.Decidable.
 Require Import Crypto.Util.Prod.
 Require Import Crypto.Util.Option.
+Require Import Crypto.Util.Sum.
 Require Import Crypto.Util.LetIn.
+Require Crypto.Util.ListUtil. (* for tests *)
 
 Section Loops.
   Context {continue_state break_state}
@@ -16,31 +20,31 @@ Section Loops.
   Definition funapp {A B} (f : A -> B) (x : A) := f x.
 
   Fixpoint loop_cps (fuel: nat) (start : continue_state)
-           {T} (ret : break_state -> T) : option T :=
+           {T} (ret : break_state -> T) : continue_state + T :=
     funapp
     (body_cps start _) (fun next =>
                       match next with
-                      | inl state => Some (ret state)
+                      | inl state => inr (ret state)
                       | inr state =>
                         match fuel with
-                        | O => None
+                        | O => inl state
                         | S fuel' =>
                           loop_cps fuel' state ret
                         end end).
   
   Fixpoint loop (fuel: nat) (start : continue_state)
-    : option break_state :=
+    : continue_state + break_state :=
     match (body start) with
-    | inl state => Some state
+    | inl state => inr state
     | inr state => 
       match fuel with
-      | O => None
+      | O => inl state
       | S fuel' => loop fuel' state
       end end.
   
   Lemma loop_break_step fuel start state :
     (body start = inl state) ->
-    loop fuel start = Some state.
+    loop fuel start = inr state.
   Proof.
     destruct fuel; simpl loop; break_match; intros; congruence.
   Qed.
@@ -48,25 +52,42 @@ Section Loops.
   Lemma loop_continue_step fuel start state :
     (body start = inr state) ->
     loop fuel start =
-    match fuel with | O => None | S fuel' => loop fuel' state end.
+    match fuel with | O => inl state | S fuel' => loop fuel' state end.
   Proof.
     destruct fuel; simpl loop; break_match; intros; congruence.
   Qed.
 
-  Definition terminates fuel start :=
-    loop fuel start <> None.
+  (* TODO: provide [invariant state] to proofs of this *)
+  Definition progress (measure : continue_state -> nat) :=
+    forall state state', body state = inr state' -> measure state' < measure state.
+  Definition terminates fuel start := forall l, loop fuel start <> inl l.
+  Lemma terminates_by_measure measure (H : progress measure) :
+    forall fuel start, measure start <= fuel -> terminates fuel start.
+  Proof.
+    induction fuel; intros;
+      repeat match goal with
+             | _ => solve [ congruence | lia ]
+             | _ => progress cbv [progress terminates] in *
+             | _ => progress cbn [loop]
+             | _ => progress break_match
+             | H : forall _ _, body _ = inr _ -> _ , Heq : body _ = inr _ |- _ => specialize (H _ _ Heq)
+             | _ => eapply IHfuel
+    end.
+  Qed.
 
   Definition loop_default fuel start default
-    : break_state := match (loop fuel start) with
-             | None => default
-             | Some result => result
-             end.
+    : break_state :=
+    sum_rect
+      (fun _ => break_state)
+      (fun _ => default)
+      (fun result => result)
+      (loop fuel start).
 
   Lemma loop_default_eq fuel start default
         (Hterm : terminates fuel start) :
-    loop fuel start = Some (loop_default fuel start default).
+    loop fuel start = inr (loop_default fuel start default).
   Proof.
-    cbv [terminates loop_default] in *; break_match; congruence.
+    cbv [terminates loop_default sum_rect] in *; break_match; congruence.
   Qed.
 
   Lemma invariant_iff fuel start default (H : terminates fuel start) P :
@@ -77,188 +98,187 @@ Section Loops.
           /\ (forall s s', body s = inl s' -> inv s -> P s')).
   Proof.
     split;
-      [ exists (fun st => exists f e, (loop f st = Some e /\ P e ))
+      [ exists (fun st => exists f e, (loop f st = inr e /\ P e ))
       | destruct 1 as [?[??]]; revert dependent start; induction fuel ];
       repeat match goal with
              | _ => solve [ trivial | congruence | eauto ] 
              | _ => progress destruct_head' @ex
              | _ => progress destruct_head' @and
              | _ => progress intros
-             | _ => progress (cbv [loop_default terminates] in * )
-             | _ => progress (cbn [loop] in * )
+             | _ => progress cbv [loop_default terminates] in *
+             | _ => progress cbn [loop] in *
              | _ => progress erewrite loop_default_eq by eassumption
              | _ => progress erewrite loop_continue_step in * by eassumption
              | _ => progress erewrite loop_break_step in * by eassumption
              | _ => progress break_match_hyps
              | _ => progress break_match
              | _ => progress eexists
+             | H1:_, c:_ |- _ => progress specialize (H1 c); congruence
              end.
-  Qed.
-
-  Lemma to_measure (measure : continue_state -> nat) :
-    (forall state state', body state = inr state' ->
-                          0 <= measure state' < measure state) ->
-    forall fuel start,
-    measure start <= fuel ->
-    terminates fuel start.
-  Proof.
-    induction fuel; intros;
-      repeat match goal with
-             | _ => solve [ congruence | lia ]
-             | _ => progress cbv [terminates]
-             | _ => progress cbn [loop]
-             | _ => progress break_match
-             | H : forall _ _, body _ = inr _ -> _ , Heq : body _ = inr _ |- _ => specialize (H _ _ Heq)
-             | _ => eapply IHfuel
-    end.
   Qed.
 End Loops.
 
 Definition by_invariant {continue_state break_state body fuel start default}
-           invariant P term invariant_start invariant_continue invariant_break
-  := proj2 (@invariant_iff continue_state break_state body fuel start default term P)
+           invariant measure P invariant_start invariant_continue invariant_break le_start progress 
+  := proj2 (@invariant_iff continue_state break_state body fuel start default (terminates_by_measure body measure progress fuel start le_start) P)
            (ex_intro _ invariant (conj invariant_start (conj invariant_continue invariant_break))).
+Arguments terminates_by_measure {_ _ _}.
                  
-Section While.
-  Context {state}
-          (test : state -> bool)
-          (body : state -> state).
+Module while.
+  Section While.
+    Context {state}
+            (test : state -> bool)
+            (body : state -> state).
 
-  Fixpoint while (fuel: nat) (s : state) {struct fuel} : option state :=
-    if test s
-    then
-      match fuel with
-      | O => None
-      | S fuel' => while fuel' (body s)
-      end
-    else Some s.
+    Fixpoint while (fuel: nat) (s : state) {struct fuel} : state :=
+      if test s
+      then
+        let s := body s in
+        match fuel with
+        | O => s
+        | S fuel' => while fuel' s
+        end
+      else s.
 
-  Section AsLoop.
-    Local Definition lbody := fun s => if test s then inr (body s) else inl s.
-    Definition while_using_loop := loop lbody.
+    Section AsLoop.
+      Local Definition lbody := fun s => if test s then inr (body s) else inl s.
 
-    Lemma while_eq_loop : forall n s, while n s = while_using_loop n s.
-    Proof.
-      induction n; intros;
-        cbv [lbody while_using_loop]; cbn [while loop]; break_match; auto.
-    Qed.
-  End AsLoop.
+      Lemma eq_loop : forall fuel start, while fuel start = loop_default lbody fuel start (while fuel start).
+      Proof.
+        induction fuel; intros;
+          cbv [lbody loop_default sum_rect id] in *;
+          cbn [while loop]; [|rewrite IHfuel]; break_match; auto.
+      Qed.
 
-  Definition while_default d f s :=
-    match while f s with
-    | None => d
-    | Some x => x
-    end.
-End While.
+      Lemma by_invariant fuel start 
+            (invariant : state -> Prop) (measure : state -> nat) (P : state -> Prop)
+            (_: invariant start)
+            (_: forall s, invariant s -> if test s then invariant (body s) else P s)
+            (_: measure start <= fuel)
+            (_: forall s, if test s then measure (body s) < measure s else True)
+        : P (while fuel start).
+      Proof.
+        rewrite eq_loop; cbv [lbody].
+        eapply (by_invariant invariant measure);
+          repeat match goal with
+                 | [ H : forall s, invariant s -> _, G: invariant ?s |- _ ] => unique pose proof (H _ G)
+                 | [ H : forall s, if ?f s then _ else _, G: ?f ?s = _ |- _ ] => unique pose proof (H s)
+                 | _ => solve [ trivial | congruence ]
+                 | _ => progress cbv [progress]
+                 | _ => progress intros
+                 | _ => progress subst
+                 | _ => progress inversion_sum
+                 | _ => progress break_match_hyps (* FIXME: this must be last? *)
+                 end.
+      Qed.
+    End AsLoop.
+  End While.
+  Arguments by_invariant {_ _ _ _ _}.
+End while.
+Notation while := while.while.
 
 Definition for2 {state} (test : state -> bool) (increment body : state -> state)
   := while test (fun s => increment (body s)). 
-Definition for2_default {state} d test increment body f s :=
-  match @for2 state test increment body f s with
-  | None => d
-  | Some x => x
-  end.
 
-Definition for3 {state} init test increment body fuel := @for2 state test increment body fuel init.
-Definition for3_default {state} d init test increment body fuel :=
-  match @for3 state init test increment body fuel with
-  | None => d
-  | Some x => x
-  end.
+Definition for3 {state} init test increment body fuel :=
+  @for2 state test increment body fuel init.
 
-Section GCD.
-  Definition gcd_step :=
-    fun '(a, b) => if Nat.ltb a b
-                   then inr (a, b-a)
-                   else if Nat.ltb b a
-                        then inr (a-b, b)
-                        else inl a.
+Module _test.
+  Section GCD.
+    Definition gcd_step :=
+      fun '(a, b) => if Nat.ltb a b
+                     then inr (a, b-a)
+                     else if Nat.ltb b a
+                          then inr (a-b, b)
+                          else inl a.
 
-  Definition gcd fuel a b := loop_default gcd_step fuel (a,b) 0.
+    Definition gcd fuel a b := loop_default gcd_step fuel (a,b) 0.
 
-  Eval cbv [gcd loop_default loop gcd_step] in (gcd 10 5 7).
-  
-  Example gcd_test : gcd 1000 28 35 = 7 := eq_refl.
+    (* Eval cbv [gcd loop_default loop gcd_step] in (gcd 10 5 7). *)
+    
+    Example gcd_test : gcd 1000 28 35 = 7 := eq_refl.
 
-  Definition gcd_step_cps
-    : (nat * nat) -> forall T, (nat + (nat * nat) -> T) -> T 
-    :=
-      fun st T ret =>
-        let a := fst st in
-        let b := snd st in
-        if Nat.ltb a b
-        then ret (inr (a, b-a))
-        else if Nat.ltb b a
-             then ret (inr (a-b, b))
-             else ret (inl a).
+    Definition gcd_step_cps
+      : (nat * nat) -> forall T, (nat + (nat * nat) -> T) -> T 
+      :=
+        fun st T ret =>
+          let a := fst st in
+          let b := snd st in
+          if Nat.ltb a b
+          then ret (inr (a, b-a))
+          else if Nat.ltb b a
+               then ret (inr (a-b, b))
+               else ret (inl a).
 
-  Definition gcd_cps fuel a b {T} (ret:nat->T)
-    := loop_cps gcd_step_cps fuel (a,b) ret.
+    Definition gcd_cps fuel a b {T} (ret:nat->T)
+      := loop_cps gcd_step_cps fuel (a,b) ret.
 
-  Example gcd_test2 : gcd_cps 1000 28 35 id = Some 7 := eq_refl.
-  
-  Eval cbv [gcd_cps loop_cps gcd_step_cps id] in (gcd_cps 2 5 7 id).
+    Example gcd_test2 : gcd_cps 1000 28 35 id = inr 7 := eq_refl.
+    
+    (* Eval cbv [gcd_cps loop_cps gcd_step_cps id] in (gcd_cps 2 5 7 id). *)
 
-End GCD.
+  End GCD.
 
-(* simple example--set all elements in a list to 0 *)
-Section ZeroLoop.
+  (* simple example--set all elements in a list to 0 *)
+  Section ZeroLoop.
+    Import Crypto.Util.ListUtil.
 
-  Definition zero_body (state : nat * list nat) :
-    list nat + (nat * list nat) :=
-    if dec (fst state < length (snd state))
-    then inr (S (fst state), set_nth (fst state) 0 (snd state))
-    else inl (snd state).
+    Definition zero_body (state : nat * list nat) :
+      list nat + (nat * list nat) :=
+      if dec (fst state < length (snd state))
+      then inr (S (fst state), set_nth (fst state) 0 (snd state))
+      else inl (snd state).
 
-  Lemma zero_body_terminates (arr : list nat) :
-    terminates zero_body (length arr) (0,arr).
-  Proof.
-    eapply to_measure with (measure :=(fun state => length (snd state) - (fst state))); cbv [zero_body]; intros until 0;
-      repeat match goal with
-             | _ => progress autorewrite with cancel_pair distr_length
-             | _ => progress subst
-             | _ => progress break_match; intros
-             | _ => congruence
-             | H: inl _ = inl _ |- _ => injection H; intros; subst; clear H
-             | H: inr _ = inr _ |- _ => injection H; intros; subst ;clear H
-             | _ => lia
-             end.
-  Qed.
+    Lemma zero_body_progress (arr : list nat) :
+      progress zero_body (fun state : nat * list nat => length (snd state) - fst state).
+    Proof.
+      cbv [zero_body progress]; intros until 0;
+        repeat match goal with
+               | _ => progress autorewrite with cancel_pair distr_length
+               | _ => progress subst
+               | _ => progress break_match; intros
+               | _ => congruence
+               | H: inl _ = inl _ |- _ => injection H; intros; subst; clear H
+               | H: inr _ = inr _ |- _ => injection H; intros; subst ;clear H
+               | _ => lia
+               end.
+    Qed.
 
-  Definition zero_loop (arr : list nat) : list nat :=
-    loop_default zero_body (length arr) (0,arr) nil.
-  
-  Definition zero_invariant (state : nat * list nat) :=
-    fst state <= length (snd state)
-    /\ forall n, n < fst state -> nth_default 0 (snd state) n = 0.
+    Definition zero_loop (arr : list nat) : list nat :=
+      loop_default zero_body (length arr) (0,arr) nil.
+    
+    Definition zero_invariant (state : nat * list nat) :=
+      fst state <= length (snd state)
+      /\ forall n, n < fst state -> nth_default 0 (snd state) n = 0.
 
-   Lemma zero_correct (arr : list nat) :
-     forall n, nth_default 0 (zero_loop arr) n = 0.
-   Proof.
-     intros. cbv [zero_loop].
-     eapply (by_invariant zero_invariant); auto using zero_body_terminates;
-       [ cbv [zero_invariant]; autorewrite with cancel_pair; split; intros; lia | ..];
-       cbv [zero_invariant zero_body];
-       intros until 0;
-       break_match; intros;
-         repeat match goal with
-                | _ => congruence
-                | H: inl _ = inl _ |- _ => injection H; intros; subst; clear H
-                | H: inr _ = inr _ |- _ => injection H; intros; subst ;clear H
-                | _ => progress split
-                | _ => progress intros
-                | _ => progress subst
-                | _ => progress (autorewrite with cancel_pair distr_length in * )
-                | _ => rewrite set_nth_nth_default by lia
-                | _ => progress break_match
-                | H : _ /\ _ |- _ => destruct H
-                | H : (_,_) = ?x |- _ =>
-                  destruct x; inversion H; subst; destruct H
-                | H : _ |- _ => apply H; lia
-                | _ => lia
-                end.
-         destruct (Compare_dec.lt_dec n (fst s)).
-         apply H1; lia.
-         apply nth_default_out_of_bounds; lia.
-   Qed.
-End ZeroLoop.
+    Lemma zero_correct (arr : list nat) :
+      forall n, nth_default 0 (zero_loop arr) n = 0.
+    Proof.
+      intros. cbv [zero_loop].
+      eapply (by_invariant zero_invariant); eauto using zero_body_progress;
+        [ cbv [zero_invariant]; autorewrite with cancel_pair; split; intros; lia | ..];
+        cbv [zero_invariant zero_body];
+        intros until 0;
+        break_match; intros;
+          repeat match goal with
+                 | _ => congruence
+                 | H: inl _ = inl _ |- _ => injection H; intros; subst; clear H
+                 | H: inr _ = inr _ |- _ => injection H; intros; subst ;clear H
+                 | _ => progress split
+                 | _ => progress intros
+                 | _ => progress subst
+                 | _ => progress (autorewrite with cancel_pair distr_length in * )
+                 | _ => rewrite set_nth_nth_default by lia
+                 | _ => progress break_match
+                 | H : _ /\ _ |- _ => destruct H
+                 | H : (_,_) = ?x |- _ =>
+                   destruct x; inversion H; subst; destruct H
+                 | H : _ |- _ => apply H; lia
+                 | _ => lia
+                 end.
+      destruct (Compare_dec.lt_dec n (fst s)).
+      apply H1; lia.
+      apply nth_default_out_of_bounds; lia.
+    Qed.
+  End ZeroLoop.
+End _test.
